Test/exceptions/TypecheckErrors.dfy
@@ -16,3 +16,33 @@ method RedeclareVar() returns (res: NatOutcome) {
     var b := MakeNatSuccess(45);
     return a;
 }
+
+trait BadOutcome1 {
+    // predicate method IsFailure() // <-- deliberately commented out
+	// function method PropagateFailure(): BadOutcome1 requires IsFailure() // <-- deliberately commented out
+	// function method Extract(): nat requires !IsFailure() // <-- deliberately commented out
+}
+
+trait BadOutcome2 {
+    predicate method IsFailure()
+	// function method PropagateFailure(): BadOutcome2 requires IsFailure() // <-- deliberately commented out
+	function method Extract(): nat requires !IsFailure()
+}
+
+trait BadOutcome3 {
+    predicate method IsFailure()
+	function method PropagateFailure(): BadOutcome3 requires IsFailure()
+	// function method Extract(): nat requires !IsFailure() // <-- deliberately commented out
+}
+
+method TestMissingMethods1(o: BadOutcome1) returns (res: BadOutcome1) {
+    var a :- o; return o; // TODO infers '?' for RHS of ':-' instead of 'BadOutcome1'
+}
+
+method TestMissingMethods2(o: BadOutcome2) returns (res: BadOutcome2) {
+    var a :- o; return o; // TODO infers 'BadOutcome2?' for RHS of ':-' instead of 'BadOutcome2' (should not infer nullable)
+}
+
+method TestMissingMethods3(o: BadOutcome3) returns (res: BadOutcome3) {
+    var a :- o; return o; // TODO infers 'BadOutcome3?' for RHS of ':-' instead of 'BadOutcome3' (should not infer nullable)
+}
